rocq/theories/TypeSystem/EnvRuntimeCapturedCallSummaryFacts.v
@@ -2441,6 +2441,41 @@ Proof.
   exists fuel'. split; [reflexivity | exact Hcallee].
 Qed.
 
+Lemma check_fn_root_shadow_captured_call_store_safe_or_no_capture_direct_component_closure_summary_sound :
+  forall env fdef,
+    check_fn_root_shadow_captured_call_store_safe_or_no_capture_direct_component_closure_summary
+      env fdef = true ->
+    callee_body_root_shadow_captured_call_store_safe_or_no_capture_direct_component_summary
+      env fdef.
+Proof.
+  intros env fdef Hcheck.
+  unfold check_fn_root_shadow_captured_call_store_safe_or_no_capture_direct_component_closure_summary
+    in Hcheck.
+  apply orb_true_iff in Hcheck as [Hcaptured | Hclosure].
+  - left. apply check_fn_root_shadow_captured_call_store_safe_summary_sound.
+    exact Hcaptured.
+  - right.
+    eapply check_fn_root_shadow_no_capture_direct_call_component_closure_head_sound.
+    exact Hclosure.
+Qed.
+
+Lemma check_env_root_shadow_captured_call_store_safe_or_no_capture_direct_component_closure_summary_ready :
+  forall env,
+    check_env_root_shadow_captured_call_store_safe_or_no_capture_direct_component_closure_summary
+      env = true ->
+    env_fns_root_shadow_captured_call_store_safe_or_no_capture_direct_component_summary_ready
+      env.
+Proof.
+  intros env Hcheck fname fdef Hlookup.
+  unfold check_env_root_shadow_captured_call_store_safe_or_no_capture_direct_component_closure_summary
+    in Hcheck.
+  destruct (lookup_fn_in_name fname (env_fns env) fdef Hlookup)
+    as [Hin _].
+  apply forallb_forall with (x := fdef) in Hcheck; [| exact Hin].
+  apply check_fn_root_shadow_captured_call_store_safe_or_no_capture_direct_component_closure_summary_sound.
+  exact Hcheck.
+Qed.
+
 Lemma check_env_root_shadow_no_capture_direct_call_component_store_safe_summary_ready :
   forall env,
     check_env_root_shadow_no_capture_direct_call_component_store_safe_summary
